examples/OCL_lib_ground.thy
@@ -1,0 +1,577 @@
+(*****************************************************************************
+ * Featherweight-OCL --- A Formal Semantics for UML-OCL Version OCL 2.4
+ *                       for the OMG Standard.
+ *                       http://www.brucker.ch/projects/hol-testgen/
+ *
+ * OCL_lib_ground.thy --- Example using the OCL library.
+ * This file is part of HOL-TestGen.
+ *
+ * Copyright (c) 2013      Universite Paris-Sud, France
+ *               2013      IRT SystemX, France
+ *
+ * All rights reserved.
+ *
+ * Redistribution and use in source and binary forms, with or without
+ * modification, are permitted provided that the following conditions are
+ * met:
+ *
+ *     * Redistributions of source code must retain the above copyright
+ *       notice, this list of conditions and the following disclaimer.
+ *
+ *     * Redistributions in binary form must reproduce the above
+ *       copyright notice, this list of conditions and the following
+ *       disclaimer in the documentation and/or other materials provided
+ *       with the distribution.
+ *
+ *     * Neither the name of the copyright holders nor the names of its
+ *       contributors may be used to endorse or promote products derived
+ *       from this software without specific prior written permission.
+ *
+ * THIS SOFTWARE IS PROVIDED BY THE COPYRIGHT HOLDERS AND CONTRIBUTORS
+ * "AS IS" AND ANY EXPRESS OR IMPLIED WARRANTIES, INCLUDING, BUT NOT
+ * LIMITED TO, THE IMPLIED WARRANTIES OF MERCHANTABILITY AND FITNESS FOR
+ * A PARTICULAR PURPOSE ARE DISCLAIMED. IN NO EVENT SHALL THE COPYRIGHT
+ * OWNER OR CONTRIBUTORS BE LIABLE FOR ANY DIRECT, INDIRECT, INCIDENTAL,
+ * SPECIAL, EXEMPLARY, OR CONSEQUENTIAL DAMAGES (INCLUDING, BUT NOT
+ * LIMITED TO, PROCUREMENT OF SUBSTITUTE GOODS OR SERVICES; LOSS OF USE,
+ * DATA, OR PROFITS; OR BUSINESS INTERRUPTION) HOWEVER CAUSED AND ON ANY
+ * THEORY OF LIABILITY, WHETHER IN CONTRACT, STRICT LIABILITY, OR TORT
+ * (INCLUDING NEGLIGENCE OR OTHERWISE) ARISING IN ANY WAY OUT OF THE USE
+ * OF THIS SOFTWARE, EVEN IF ADVISED OF THE POSSIBILITY OF SUCH DAMAGE.
+ ******************************************************************************)
+(* $Id:$ *)
+
+header{* Gogolla's challenge on Sets (1/2) *}
+
+theory
+  OCL_lib_ground
+imports
+  "../src/OCL_lib"
+begin
+
+(*
+Sequence{6,8}->iterate(i;r1:Sequence(Integer)=Sequence{9}|
+  r1->iterate(j;r2:Sequence(Integer)=r1|
+    r2->including(0)->including(i)->including(j)))
+*)
+text{* In order to analyze the performance of the library,
+we propose in this section to execute and normalize a not trivial OCL expression.
+Consider for instance this ground term:
+@{term "Set{\<six>,\<eight>}->iterate(i;r1=Set{\<nine>}|
+  r1->iterate(j;r2=r1|
+    r2->including(\<zero>)->including(i)->including(j)))"}.
+Starting from a set of numbers, this complex expression finally involves only two combinators:
+1) @{term OclIterate\<^isub>S\<^isub>e\<^isub>t}, and
+2) @{term OclIncluding}.
+
+As there is no removing, we conjecture that the final result should be equal to the set
+containing all ground numbers appearing in the expression: that is @{term \<six>}, @{term \<eight>}, @{term \<nine>}, @{term \<zero>}. *}
+(* text{*(modulo ordering and duplication for sequences)*} *)
+
+text{* The following part sets up the necessary requirement towards an automatic execution.
+The goal is to normalize a general term composed of a set of numbers applied to an arbitrary nesting of
+@{term OclIterate\<^isub>S\<^isub>e\<^isub>t} and @{term OclIncluding}.
+One solution is to rawly compute the initial term by following a call by value strategy or by need.
+However for efficiency reasons, we present in the next subsections some algebraic properties on sets
+that would shortcut the number of reduction steps, by reaching optimaly a normal form. *}
+
+section{* Introduction *}
+
+text{* Besides the @{term invalid} exception element, the other important concept that
+characterizes OCL sets in our formalization is the finiteness property.
+Since the iteration could only be performed on finite sets, the definition of @{term OclIterate\<^isub>S\<^isub>e\<^isub>t}
+contains as prerequisite a check that the given argument is finite. If it is the case,
+@{term Finite_Set.fold} is then called internally to execute the iteration. *}
+
+text{* Recall that our goal is to provide a generic solution to the Gogolla's challenge,
+in the sense that we focus on an arbitrary list of nested @{term OclIterate\<^isub>S\<^isub>e\<^isub>t} combinators.
+A naive approach for simplifying such huge expression would be to repeatedly rewrite with
+@{term OclIterate\<^isub>S\<^isub>e\<^isub>t_including}.
+However, @{term OclIterate\<^isub>S\<^isub>e\<^isub>t_including} contains @{term "comp_fun_commute F"} as hypothesis
+and this one is generally difficult to prove. Indeed, the easiest case would be when simplifying
+the outermost @{term OclIterate\<^isub>S\<^isub>e\<^isub>t} since the overall expression is ground. But for the others inner nested
+@{term OclIterate\<^isub>S\<^isub>e\<^isub>t}, the @{term "F"} function could have as free variable a set
+where its validity, definedness and finiteness are unknown --
+and the finiteness is precisely required for all sets occuring
+in a chain of @{term OclIterate\<^isub>S\<^isub>e\<^isub>t} nested term. *}
+
+text{* Thus we propose to write an Isabelle locale similar as the locale @{term "comp_fun_commute"}
+but containing the additional properties that sets should fulfill
+while traveling through the nested @{term OclIterate\<^isub>S\<^isub>e\<^isub>t}.
+For reusability, these properties will be abstractly regrouped in @{term "is_int"} (representing ground value in a set, like integer)
+and @{term "all_defined"} (representing ground sets). *}
+
+definition "is_int x \<equiv> \<forall> \<tau>. \<tau> \<Turnstile> \<upsilon> x \<and> (\<forall>\<tau>0. x \<tau> = x \<tau>0)"
+
+lemma int_is_valid : "\<And>x. is_int x \<Longrightarrow> \<tau> \<Turnstile> \<upsilon> x"
+by (metis foundation18' is_int_def)
+
+definition "all_int_set S \<equiv> finite S \<and> (\<forall>x\<in>S. is_int x)"
+definition "all_int \<tau> S \<equiv> (\<tau> \<Turnstile> \<delta> S) \<and> all_int_set \<lceil>\<lceil>Rep_Set_0 (S \<tau>)\<rceil>\<rceil>"
+definition "all_defined_set \<tau> S \<equiv> finite S \<and> (\<forall>x\<in>S. (\<tau> \<Turnstile> \<upsilon> (\<lambda>_. x)))"
+definition "all_defined_set' \<tau> S \<equiv> finite S"
+definition "all_defined \<tau> S \<equiv> (\<tau> \<Turnstile> \<delta> S) \<and> all_defined_set' \<tau> \<lceil>\<lceil>Rep_Set_0 (S \<tau>)\<rceil>\<rceil>"
+
+lemma all_def_to_all_int : "\<And>\<tau>. all_defined \<tau> S \<Longrightarrow>
+                                all_int_set ((\<lambda>a \<tau>. a) ` \<lceil>\<lceil>Rep_Set_0 (S \<tau>)\<rceil>\<rceil>)"
+ apply(simp add: all_defined_def, erule conjE, frule Set_inv_lemma)
+ apply(simp add: all_defined_def all_defined_set'_def all_int_set_def is_int_def defined_def OclValid_def)
+by (metis (no_types) OclValid_def foundation18' true_def Set_inv_lemma')
+
+term "all_defined \<tau> (f \<zero> Set{\<zero>}) = (all_defined \<tau> Set{\<zero>})"
+ (* we check here that all_defined could at least be applied to some useful value
+    (i.e. we examine the type of all_defined) *)
+
+lemma int_trivial : "is_int (\<lambda>_. \<lfloor>a\<rfloor>)" by(simp add: is_int_def OclValid_def valid_def bot_fun_def bot_option_def)
+
+lemma EQ_sym : "(x::(_, _) Set) = y \<Longrightarrow> \<tau> \<Turnstile> \<upsilon> x \<Longrightarrow> \<tau> \<Turnstile> (x \<doteq> y)"
+  apply(simp add: OclValid_def)
+done
+
+lemma StrictRefEq\<^isub>S\<^isub>e\<^isub>t_L_subst1 : "cp P \<Longrightarrow> \<tau> \<Turnstile> \<upsilon> x \<Longrightarrow> \<tau> \<Turnstile> \<upsilon> y \<Longrightarrow> \<tau> \<Turnstile> \<upsilon> P x \<Longrightarrow> \<tau> \<Turnstile> \<upsilon> P y \<Longrightarrow> \<tau> \<Turnstile> (x::('\<AA>,'\<alpha>::null)Set) \<doteq> y \<Longrightarrow> \<tau> \<Turnstile> (P x ::('\<AA>,'\<alpha>::null)Set) \<doteq> P y"
+ apply(simp only: StrictRefEq\<^isub>S\<^isub>e\<^isub>t OclValid_def)
+ apply(split split_if_asm)
+ apply(simp add: StrongEq_L_subst1[simplified OclValid_def])
+by (simp add: invalid_def bot_option_def true_def)
+
+lemma abs_rep_simp :
+ assumes S_all_def : "all_defined \<tau> (S :: ('\<AA>, 'a option option) Set)"
+   shows "Abs_Set_0 \<lfloor>\<lfloor>\<lceil>\<lceil>Rep_Set_0 (S \<tau>)\<rceil>\<rceil>\<rfloor>\<rfloor> = S \<tau>"
+by(rule abs_rep_simp', simp add: assms[simplified all_defined_def])
+
+lemma cp_all_def : "all_defined \<tau> f = all_defined \<tau>' (\<lambda>_. f \<tau>)"
+  apply(simp add: all_defined_def all_defined_set'_def OclValid_def)
+  apply(subst cp_defined)
+by (metis (no_types) OclValid_def foundation16)
+
+lemma cp_all_def' : "(\<forall>\<tau>. all_defined \<tau> f) = (\<forall>\<tau> \<tau>'. all_defined \<tau>' (\<lambda>_. f \<tau>))"
+ apply(rule iffI)
+ apply(rule allI) apply(erule_tac x = \<tau> in allE) apply(rule allI)
+ apply(simp add: cp_all_def[THEN iffD1])
+ apply(subst cp_all_def, blast)
+done
+
+lemma S_lift :
+ assumes S_all_def : "all_defined (\<tau> :: '\<AA> st) S"
+   shows "\<exists>S'. (\<lambda>a (_::'\<AA> st). a) ` \<lceil>\<lceil>Rep_Set_0 (S \<tau>)\<rceil>\<rceil> = (\<lambda>a (_::'\<AA> st). \<lfloor>a\<rfloor>) ` S'"
+by(rule S_lift', simp add: assms[simplified all_defined_def])
+
+lemma destruct_int : "is_int i \<Longrightarrow> \<exists>! j. i = (\<lambda>_. j)"
+ proof - fix \<tau> show "is_int i \<Longrightarrow> ?thesis"
+  apply(rule_tac a = "i \<tau>" in ex1I)
+  apply(rule ext, simp add: is_int_def)
+  apply (metis surj_pair)
+  apply(simp)
+ done
+ apply_end(simp)
+qed
+
+section{* Properties: mtSet *}
+
+lemma mtSet_all_def : "all_defined \<tau> Set{}"
+proof -
+ have B : "\<lfloor>\<lfloor>{}\<rfloor>\<rfloor> \<in> {X. X = bot \<or> X = null \<or> (\<forall>x\<in>\<lceil>\<lceil>X\<rceil>\<rceil>. x \<noteq> bot)}" by(simp add: mtSet_def)
+ show ?thesis
+  apply(simp add: all_defined_def all_defined_set'_def mtSet_def Abs_Set_0_inverse B)
+ by (metis (no_types) foundation16 mtSet_def mtSet_defined transform1)
+qed
+
+lemma cp_mtSet : "\<And>x. Set{} = (\<lambda>_. Set{} x)"
+by (metis (hide_lams, no_types) mtSet_def)
+
+section{* Properties: OclIncluding *}
+
+subsection{* Identity *}
+
+lemma including_id' : "all_defined \<tau> (S:: ('\<AA>, 'a option option) Set) \<Longrightarrow>
+                       x \<in> \<lceil>\<lceil>Rep_Set_0 (S \<tau>)\<rceil>\<rceil> \<Longrightarrow>
+                       S->including(\<lambda>\<tau>. x) \<tau> = S \<tau>"
+proof -
+ have discr_eq_invalid_true : "\<And>\<tau>. (invalid \<tau> = true \<tau>) = False" by (metis bot_option_def invalid_def option.simps(2) true_def)
+
+ have all_defined1 : "\<And>r2. all_defined \<tau> r2 \<Longrightarrow> \<tau> \<Turnstile> \<delta> r2" by(simp add: all_defined_def)
+
+ show "               all_defined \<tau> S \<Longrightarrow>
+                      x \<in> \<lceil>\<lceil>Rep_Set_0 (S \<tau>)\<rceil>\<rceil> \<Longrightarrow>
+                      ?thesis"
+  apply(simp add: OclIncluding_def all_defined1[simplified OclValid_def] OclValid_def insert_absorb abs_rep_simp del: StrictRefEq\<^isub>S\<^isub>e\<^isub>t_exec)
+ by (metis OCL_core.bot_fun_def all_defined_def foundation18' valid_def Set_inv_lemma')
+qed
+
+lemma including_id :
+ assumes S_all_def : "\<And>\<tau>. all_defined \<tau> (S :: ('\<AA>, 'a option option) Set)"
+   shows "            \<forall>\<tau>. x \<in> \<lceil>\<lceil>Rep_Set_0 (S \<tau>)\<rceil>\<rceil> \<Longrightarrow>
+                      S->including(\<lambda>\<tau>. x) = S"
+proof -
+ have all_defined1 : "\<And>r2 \<tau>. all_defined \<tau> r2 \<Longrightarrow> \<tau> \<Turnstile> \<delta> r2" by(simp add: all_defined_def)
+
+ have x_val : "\<And>\<tau>. (\<forall>\<tau>. x \<in> \<lceil>\<lceil>Rep_Set_0 (S \<tau>)\<rceil>\<rceil>) \<Longrightarrow>
+               \<tau> \<Turnstile> \<upsilon> (\<lambda>\<tau>. x)"
+  apply(insert S_all_def)
+  apply(simp add: all_defined_def all_defined_set_def)
+ by (metis (no_types) foundation18' Set_inv_lemma')
+
+ show "               (\<forall>\<tau>. x \<in> \<lceil>\<lceil>Rep_Set_0 (S \<tau>)\<rceil>\<rceil>) \<Longrightarrow>
+                      ?thesis"
+  apply(rule ext, rename_tac \<tau>', simp add: OclIncluding_def)
+  apply(subst insert_absorb) apply (metis (full_types) surj_pair)
+  apply(subst abs_rep_simp, simp add: S_all_def, simp)
+  proof - fix \<tau>' show "\<forall>a b. x \<in> \<lceil>\<lceil>Rep_Set_0 (S (a, b))\<rceil>\<rceil> \<Longrightarrow> ((\<delta> S) \<tau>' = true \<tau>' \<longrightarrow> (\<upsilon> (\<lambda>\<tau>. x)) \<tau>' \<noteq> true \<tau>') \<longrightarrow> \<bottom> = S \<tau>'"
+  apply(frule x_val[simplified, where \<tau> = \<tau>'])
+  apply(insert S_all_def[where \<tau> = \<tau>'])
+  apply(subst all_defined1[simplified OclValid_def], simp)
+  by (metis OclValid_def)
+ qed
+ apply_end(simp)
+qed
+
+subsection{* Commutativity *}
+
+lemma including_swap_ :
+ assumes S_def : "\<tau> \<Turnstile> \<delta> S"
+     and i_val : "\<tau> \<Turnstile> \<upsilon> i"
+     and j_val : "\<tau> \<Turnstile> \<upsilon> j"
+   shows "\<tau> \<Turnstile> ((S :: ('\<AA>, int option option) Set)->including(i)->including(j) \<doteq> (S->including(j)->including(i)))"
+proof -
+
+ have OclAnd_true : "\<And>a b. \<tau> \<Turnstile> a \<Longrightarrow> \<tau> \<Turnstile> b \<Longrightarrow> \<tau> \<Turnstile> a and b"
+ by (simp add: foundation10 foundation6)
+
+ have OclIf_true'' : "\<And>P B\<^isub>1 B\<^isub>2. \<tau> \<Turnstile> P \<Longrightarrow> \<tau> \<Turnstile> B\<^isub>1 \<Longrightarrow> \<tau> \<Turnstile> if P then B\<^isub>1 else B\<^isub>2 endif"
+ by (metis OclIf_true' OclValid_def)
+
+ have OclIf_false'' : "\<And>P B\<^isub>1 B\<^isub>2. \<tau> \<Turnstile> \<delta> P \<Longrightarrow> \<not> (\<tau> \<Turnstile> P) \<Longrightarrow> \<tau> \<Turnstile> B\<^isub>2 \<Longrightarrow> \<tau> \<Turnstile> if P then B\<^isub>1 else B\<^isub>2 endif"
+ by (metis OclIf_def OclValid_def)
+
+ have discr_eq_false_true : "\<And>\<tau>. (false \<tau> = true \<tau>) = False" by (metis OclValid_def foundation2)
+ have discr_eq_null_true : "\<And>\<tau>. (null \<tau> = true \<tau>) = False" by (metis OclValid_def foundation4)
+ have discr_eq_bot1_true : "\<And>\<tau>. (\<bottom> \<tau> = true \<tau>) = False" by (metis defined3 defined_def discr_eq_false_true)
+ have discr_neq_true_false : "\<And>\<tau>. (true \<tau> \<noteq> false \<tau>) = True" by (metis discr_eq_false_true)
+ have discr_neq_true_bot : "\<And>\<tau>. (true \<tau> \<noteq> bot \<tau>) = True" by (metis discr_eq_bot1_true)
+ have discr_neq_true_null : "\<And>\<tau>. (true \<tau> \<noteq> null \<tau>) = True" by (metis discr_eq_null_true)
+
+ have forall_includes2 : "\<And>a b. \<tau> \<Turnstile> \<upsilon> a \<Longrightarrow> \<tau> \<Turnstile> \<upsilon> b \<Longrightarrow> \<tau> \<Turnstile> \<delta> S \<Longrightarrow> \<tau> \<Turnstile> (OclForall S (OclIncludes (S->including(a)->including(b))))"
+ proof -
+  have consist : "\<And>x. (\<delta> S) \<tau> = true \<tau> \<Longrightarrow> x \<in> \<lceil>\<lceil>Rep_Set_0 (S \<tau>)\<rceil>\<rceil> \<Longrightarrow> (\<upsilon> (\<lambda>_. x)) \<tau> = true \<tau>"
+  by(simp add: Set_inv_lemma'[simplified OclValid_def])
+  show "\<And>a b. \<tau> \<Turnstile> \<upsilon> a \<Longrightarrow> \<tau> \<Turnstile> \<upsilon> b \<Longrightarrow> \<tau> \<Turnstile> \<delta> S \<Longrightarrow> ?thesis a b"
+   apply(simp add: OclForall_def OclValid_def discr_eq_false_true discr_eq_bot1_true discr_eq_null_true)
+   apply(subgoal_tac "\<forall>x\<in>\<lceil>\<lceil>Rep_Set_0 (S \<tau>)\<rceil>\<rceil>. (S->including(a)->including(b)->includes((\<lambda>_. x))) \<tau> = true \<tau>")
+   apply(simp add: discr_neq_true_null discr_neq_true_bot discr_neq_true_false)
+   apply(rule ballI)
+   apply(rule including_includes[simplified OclValid_def], simp, rule consist, simp, simp)+
+   apply(frule Set_inv_lemma'[simplified OclValid_def]) apply assumption
+   apply(simp add: OclIncludes_def true_def)
+  done
+ qed
+
+ show "\<tau> \<Turnstile> \<delta> S \<Longrightarrow> \<tau> \<Turnstile> \<upsilon> i \<Longrightarrow> \<tau> \<Turnstile> \<upsilon> j \<Longrightarrow> ?thesis"
+  apply(simp only: StrictRefEq\<^isub>S\<^isub>e\<^isub>t_exec)
+  (* *)
+  apply(subst OclIf_true'', simp_all add: foundation10 foundation6 del: forall_set_including_exec)+
+  apply(subst (1 2) forall_set_including_exec, simp add: cp_OclIncludes1, simp add: cp_OclIncludes1)+
+  apply(subst OclAnd_true)
+  (* *)
+  apply(subst OclIf_true'', simp_all add: foundation10 foundation6 del: forall_set_including_exec)+
+  apply(subst OclAnd_true)
+  apply(subst OclIf_true'', simp_all add: foundation10 foundation6 del: forall_set_including_exec)
+  apply(case_tac "\<tau> \<Turnstile> (i \<doteq> j)")
+  apply(subst OclIf_true'', simp_all add: foundation10 foundation6 del: forall_set_including_exec)
+  apply(subst OclIf_false'', simp_all add: StrictRefEq\<^isub>I\<^isub>n\<^isub>t\<^isub>e\<^isub>g\<^isub>e\<^isub>r_defined_args_valid)
+  apply( subst OclAnd_true
+       | subst OclIf_true'', simp_all add: foundation10 foundation6 del: forall_set_including_exec)+
+  apply(simp add: forall_includes2)
+  (* *)
+  apply(subst OclIf_true'', simp_all add: foundation10 foundation6 del: forall_set_including_exec)+
+  apply(subst OclAnd_true)
+  apply(subst OclIf_true'', simp_all add: foundation10 foundation6 del: forall_set_including_exec)
+  apply(case_tac "\<tau> \<Turnstile> (j \<doteq> i)")
+  apply(subst OclIf_true'', simp_all add: foundation10 foundation6 del: forall_set_including_exec)
+  apply(subst OclIf_false'', simp_all add: StrictRefEq\<^isub>I\<^isub>n\<^isub>t\<^isub>e\<^isub>g\<^isub>e\<^isub>r_defined_args_valid)
+  apply( subst OclAnd_true
+       | subst OclIf_true'', simp_all add: foundation10 foundation6 del: forall_set_including_exec)+
+  apply(simp add: forall_includes2)
+ done
+ apply_end(simp_all add: assms)
+qed
+
+lemma including_swap' : "\<tau> \<Turnstile> \<delta> S \<Longrightarrow> \<tau> \<Turnstile> \<upsilon> i \<Longrightarrow> \<tau> \<Turnstile> \<upsilon> j \<Longrightarrow> ((S :: ('\<AA>, int option option) Set)->including(i)->including(j) \<tau> = (S->including(j)->including(i)) \<tau>)"
+ apply(frule including_swap_[where i = i and j = j], simp_all del: StrictRefEq\<^isub>S\<^isub>e\<^isub>t_exec)
+ apply(simp add: StrictRefEq\<^isub>S\<^isub>e\<^isub>t OclValid_def del: StrictRefEq\<^isub>S\<^isub>e\<^isub>t_exec)
+ apply(subgoal_tac "(\<delta> S and \<upsilon> i and \<upsilon> j) \<tau> = true \<tau> \<and> (\<delta> S and \<upsilon> j and \<upsilon> i) \<tau> = true \<tau>")
+  prefer 2
+  apply(metis OclValid_def foundation3)
+ apply(simp add: StrongEq_def true_def)
+done
+
+lemma including_swap : "\<forall>\<tau>. \<tau> \<Turnstile> \<delta> S \<Longrightarrow> \<forall>\<tau>. \<tau> \<Turnstile> \<upsilon> i \<Longrightarrow> \<forall>\<tau>. \<tau> \<Turnstile> \<upsilon> j \<Longrightarrow> ((S :: ('\<AA>, int option option) Set)->including(i)->including(j) = (S->including(j)->including(i)))"
+ apply(rule ext, rename_tac \<tau>)
+ apply(erule_tac x = \<tau> in allE)+
+ apply(frule including_swap_[where i = i and j = j], simp_all del: StrictRefEq\<^isub>S\<^isub>e\<^isub>t_exec)
+ apply(simp add: StrictRefEq\<^isub>S\<^isub>e\<^isub>t OclValid_def del: StrictRefEq\<^isub>S\<^isub>e\<^isub>t_exec)
+ apply(subgoal_tac "(\<delta> S and \<upsilon> i and \<upsilon> j) \<tau> = true \<tau> \<and> (\<delta> S and \<upsilon> j and \<upsilon> i) \<tau> = true \<tau>")
+  prefer 2
+  apply(metis OclValid_def foundation3)
+ apply(simp add: StrongEq_def true_def)
+done
+
+subsection{* Congruence *}
+
+lemma including_subst_set : "(s::('\<AA>,'a::null)Set) = t \<Longrightarrow> s->including(x) = (t->including(x))"
+by(simp)
+
+lemma including_subst_set' :
+shows "\<tau> \<Turnstile> \<delta> s \<Longrightarrow> \<tau> \<Turnstile> \<delta> t \<Longrightarrow> \<tau> \<Turnstile> \<upsilon> x \<Longrightarrow> \<tau> \<Turnstile> ((s::('\<AA>,'a::null)Set) \<doteq> t) \<Longrightarrow> \<tau> \<Turnstile> (s->including(x) \<doteq> (t->including(x)))"
+proof -
+ have cp: "cp (\<lambda>s. (s->including(x)))"
+  apply(simp add: cp_def, subst cp_OclIncluding)
+ by (rule_tac x = "(\<lambda>xab ab. ((\<lambda>_. xab)->including(\<lambda>_. x ab)) ab)" in exI, simp)
+
+ show "\<tau> \<Turnstile> \<delta> s \<Longrightarrow> \<tau> \<Turnstile> \<delta> t \<Longrightarrow> \<tau> \<Turnstile> \<upsilon> x \<Longrightarrow> \<tau> \<Turnstile> (s \<doteq> t) \<Longrightarrow> ?thesis"
+  apply(rule_tac P = "\<lambda>s. (s->including(x))" in StrictRefEq\<^isub>S\<^isub>e\<^isub>t_L_subst1)
+  apply(rule cp)
+  apply(simp add: foundation20) apply(simp add: foundation20)
+  apply (simp add: foundation10 foundation6)+
+ done
+qed
+
+lemma including_subst_set'' : "\<tau> \<Turnstile> \<delta> s \<Longrightarrow> \<tau> \<Turnstile> \<delta> t \<Longrightarrow> \<tau> \<Turnstile> \<upsilon> x \<Longrightarrow> (s::('\<AA>,'a::null)Set) \<tau> = t \<tau> \<Longrightarrow> s->including(x) \<tau> = (t->including(x)) \<tau>"
+ apply(frule including_subst_set'[where s = s and t = t and x = x], simp_all del: StrictRefEq\<^isub>S\<^isub>e\<^isub>t_exec)
+ apply(simp add: StrictRefEq\<^isub>S\<^isub>e\<^isub>t OclValid_def del: StrictRefEq\<^isub>S\<^isub>e\<^isub>t_exec)
+ apply (metis (hide_lams, no_types) OclValid_def foundation20 foundation22)
+by (metis cp_OclIncluding)
+
+
+subsection{* all defined (construction) *}
+
+lemma cons_all_def :
+  assumes S_all_def : "\<And>\<tau>. all_defined \<tau> S"
+  assumes x_val : "\<And>\<tau>. \<tau> \<Turnstile> \<upsilon> x"
+    shows "all_defined \<tau> S->including(x)"
+proof -
+
+ have discr_eq_false_true : "\<And>\<tau>. (false \<tau> = true \<tau>) = False" by (metis OclValid_def foundation2)
+
+ have all_defined1 : "\<And>r2 \<tau>. all_defined \<tau> r2 \<Longrightarrow> \<tau> \<Turnstile> \<delta> r2" by(simp add: all_defined_def)
+
+ have A : "\<bottom> \<in> {X. X = bot \<or> X = null \<or> (\<forall>x\<in>\<lceil>\<lceil>X\<rceil>\<rceil>. x \<noteq> bot)}" by(simp add: bot_option_def)
+ have B : "\<lfloor>\<bottom>\<rfloor> \<in> {X. X = bot \<or> X = null \<or> (\<forall>x\<in>\<lceil>\<lceil>X\<rceil>\<rceil>. x \<noteq> bot)}" by(simp add: null_option_def bot_option_def)
+
+ have C : "\<And>\<tau>. \<lfloor>\<lfloor>insert (x \<tau>) \<lceil>\<lceil>Rep_Set_0 (S \<tau>)\<rceil>\<rceil>\<rfloor>\<rfloor> \<in> {X. X = bot \<or> X = null \<or> (\<forall>x\<in>\<lceil>\<lceil>X\<rceil>\<rceil>. x \<noteq> bot)}"
+  proof - fix \<tau> show "?thesis \<tau>"
+          apply(insert S_all_def[simplified all_defined_def, THEN conjunct1, of \<tau>]
+                       x_val, frule Set_inv_lemma)
+          apply(simp add: foundation18 invalid_def)
+          done
+  qed
+
+ have G1 : "\<And>\<tau>. Abs_Set_0 \<lfloor>\<lfloor>insert (x \<tau>) \<lceil>\<lceil>Rep_Set_0 (S \<tau>)\<rceil>\<rceil>\<rfloor>\<rfloor> \<noteq> Abs_Set_0 None"
+  proof - fix \<tau> show "?thesis \<tau>"
+          apply(insert C, simp)
+          apply(simp add:  S_all_def[simplified all_defined_def, THEN conjunct1, of \<tau>] x_val[of \<tau>] A Abs_Set_0_inject B C OclValid_def Rep_Set_0_cases Rep_Set_0_inverse bot_Set_0_def bot_option_def insert_compr insert_def not_Some_eq null_Set_0_def null_option_def)
+  done
+ qed
+
+ have G2 : "\<And>\<tau>. Abs_Set_0 \<lfloor>\<lfloor>insert (x \<tau>) \<lceil>\<lceil>Rep_Set_0 (S \<tau>)\<rceil>\<rceil>\<rfloor>\<rfloor> \<noteq> Abs_Set_0 \<lfloor>None\<rfloor>"
+  proof - fix \<tau> show "?thesis \<tau>"
+          apply(insert C, simp)
+          apply(simp add:  S_all_def[simplified all_defined_def, THEN conjunct1, of \<tau>] x_val[of \<tau>] A Abs_Set_0_inject B C OclValid_def Rep_Set_0_cases Rep_Set_0_inverse bot_Set_0_def bot_option_def insert_compr insert_def not_Some_eq null_Set_0_def null_option_def)
+  done
+ qed
+
+ have G : "\<And>\<tau>. (\<delta> (\<lambda>_. Abs_Set_0 \<lfloor>\<lfloor>insert (x \<tau>) \<lceil>\<lceil>Rep_Set_0 (S \<tau>)\<rceil>\<rceil>\<rfloor>\<rfloor>)) \<tau> = true \<tau>"
+  proof - fix \<tau> show "?thesis \<tau>"
+          apply(auto simp: OclValid_def false_def true_def defined_def
+                           bot_fun_def bot_Set_0_def null_fun_def null_Set_0_def G1 G2)
+  done
+ qed
+
+ have invert_all_defined_aux : "(\<tau> \<Turnstile>(\<delta> S)) \<Longrightarrow> (\<tau> \<Turnstile>(\<upsilon> x)) \<Longrightarrow> \<lfloor>\<lfloor>insert (x \<tau>) \<lceil>\<lceil>Rep_Set_0 (S \<tau>)\<rceil>\<rceil>\<rfloor>\<rfloor> \<in> {X. X = bot \<or> X = null \<or> (\<forall>x\<in>\<lceil>\<lceil>X\<rceil>\<rceil>. x \<noteq> bot)}"
+          apply(frule Set_inv_lemma)
+          apply(simp add: foundation18 invalid_def)
+          done
+
+  show ?thesis
+   apply(subgoal_tac "\<tau> \<Turnstile> \<upsilon> x") prefer 2 apply(simp add: x_val)
+   apply(simp add: all_defined_def OclIncluding_def OclValid_def)
+   apply(simp add: x_val[simplified OclValid_def] S_all_def[simplified all_defined_def OclValid_def])
+   apply(insert Abs_Set_0_inverse[OF invert_all_defined_aux]
+                S_all_def[simplified all_defined_def, of \<tau>]
+                x_val[of \<tau>], simp)
+   apply(simp add: cp_defined[of "\<lambda>\<tau>. Abs_Set_0 \<lfloor>\<lfloor>insert (x \<tau>) \<lceil>\<lceil>Rep_Set_0 (S \<tau>)\<rceil>\<rceil>\<rfloor>\<rfloor>"])
+   apply(simp add: all_defined_set'_def OclValid_def)
+   apply(simp add: cp_valid[symmetric] x_val[simplified OclValid_def])
+   apply(rule G)
+ done
+qed
+
+lemma cons_all_def' :
+  assumes S_all_def : "all_defined \<tau> S"
+  assumes x_val : "\<tau> \<Turnstile> \<upsilon> x"
+    shows "all_defined \<tau> (S->including(x))"
+proof -
+
+ have discr_eq_false_true : "\<And>\<tau>. (false \<tau> = true \<tau>) = False" by (metis OclValid_def foundation2)
+
+ have all_defined1 : "\<And>r2 \<tau>. all_defined \<tau> r2 \<Longrightarrow> \<tau> \<Turnstile> \<delta> r2" by(simp add: all_defined_def)
+
+ have A : "\<bottom> \<in> {X. X = bot \<or> X = null \<or> (\<forall>x\<in>\<lceil>\<lceil>X\<rceil>\<rceil>. x \<noteq> bot)}" by(simp add: bot_option_def)
+ have B : "\<lfloor>\<bottom>\<rfloor> \<in> {X. X = bot \<or> X = null \<or> (\<forall>x\<in>\<lceil>\<lceil>X\<rceil>\<rceil>. x \<noteq> bot)}" by(simp add: null_option_def bot_option_def)
+
+ have C : "\<lfloor>\<lfloor>insert (x \<tau>) \<lceil>\<lceil>Rep_Set_0 (S \<tau>)\<rceil>\<rceil>\<rfloor>\<rfloor> \<in> {X. X = bot \<or> X = null \<or> (\<forall>x\<in>\<lceil>\<lceil>X\<rceil>\<rceil>. x \<noteq> bot)}"
+          apply(insert S_all_def[simplified all_defined_def, THEN conjunct1]
+                       x_val, frule Set_inv_lemma)
+          apply(simp add: foundation18 invalid_def)
+          done
+
+ have G1 : "Abs_Set_0 \<lfloor>\<lfloor>insert (x \<tau>) \<lceil>\<lceil>Rep_Set_0 (S \<tau>)\<rceil>\<rceil>\<rfloor>\<rfloor> \<noteq> Abs_Set_0 None"
+          apply(insert C, simp)
+          apply(simp add:  S_all_def[simplified all_defined_def, THEN conjunct1] x_val A Abs_Set_0_inject B C OclValid_def Rep_Set_0_cases Rep_Set_0_inverse bot_Set_0_def bot_option_def insert_compr insert_def not_Some_eq null_Set_0_def null_option_def)
+  done
+
+ have G2 : "Abs_Set_0 \<lfloor>\<lfloor>insert (x \<tau>) \<lceil>\<lceil>Rep_Set_0 (S \<tau>)\<rceil>\<rceil>\<rfloor>\<rfloor> \<noteq> Abs_Set_0 \<lfloor>None\<rfloor>"
+          apply(insert C, simp)
+          apply(simp add:  S_all_def[simplified all_defined_def, THEN conjunct1] x_val A Abs_Set_0_inject B C OclValid_def Rep_Set_0_cases Rep_Set_0_inverse bot_Set_0_def bot_option_def insert_compr insert_def not_Some_eq null_Set_0_def null_option_def)
+  done
+
+ have G : "(\<delta> (\<lambda>_. Abs_Set_0 \<lfloor>\<lfloor>insert (x \<tau>) \<lceil>\<lceil>Rep_Set_0 (S \<tau>)\<rceil>\<rceil>\<rfloor>\<rfloor>)) \<tau> = true \<tau>"
+          apply(auto simp: OclValid_def false_def true_def defined_def
+                           bot_fun_def bot_Set_0_def null_fun_def null_Set_0_def G1 G2)
+  done
+
+ have invert_all_defined_aux : "(\<tau> \<Turnstile>(\<delta> S)) \<Longrightarrow> (\<tau> \<Turnstile>(\<upsilon> x)) \<Longrightarrow> \<lfloor>\<lfloor>insert (x \<tau>) \<lceil>\<lceil>Rep_Set_0 (S \<tau>)\<rceil>\<rceil>\<rfloor>\<rfloor> \<in> {X. X = bot \<or> X = null \<or> (\<forall>x\<in>\<lceil>\<lceil>X\<rceil>\<rceil>. x \<noteq> bot)}"
+          apply(frule Set_inv_lemma)
+          apply(simp add: foundation18 invalid_def)
+          done
+  show ?thesis
+   apply(subgoal_tac "\<tau> \<Turnstile> \<upsilon> x") prefer 2 apply(simp add: x_val)
+   apply(simp add: all_defined_def OclIncluding_def OclValid_def)
+   apply(simp add: x_val[simplified OclValid_def] S_all_def[simplified all_defined_def OclValid_def])
+   apply(insert Abs_Set_0_inverse[OF invert_all_defined_aux]
+                S_all_def[simplified all_defined_def]
+                x_val, simp)
+   apply(simp add: cp_defined[of "\<lambda>\<tau>. if (\<delta> S) \<tau> = true \<tau> \<and> (\<upsilon> x) \<tau> = true \<tau> then Abs_Set_0 \<lfloor>\<lfloor>\<lceil>\<lceil>Rep_Set_0 (S \<tau>)\<rceil>\<rceil> \<union> {x \<tau>}\<rfloor>\<rfloor> else \<bottom>"])
+   apply(simp add: all_defined_set'_def OclValid_def)
+   apply(simp add: cp_valid[symmetric] x_val[simplified OclValid_def])
+   apply(rule G)
+ done
+qed
+
+subsection{* all defined (inversion) *}
+
+lemma invert_all_defined : "all_defined \<tau> (S->including(x)) \<Longrightarrow> \<tau> \<Turnstile> \<upsilon> x \<and> all_defined \<tau> S"
+ proof -
+ have invert_all_defined_aux : "(\<tau> \<Turnstile>(\<delta> S)) \<Longrightarrow> (\<tau> \<Turnstile>(\<upsilon> x)) \<Longrightarrow> \<lfloor>\<lfloor>insert (x \<tau>) \<lceil>\<lceil>Rep_Set_0 (S \<tau>)\<rceil>\<rceil>\<rfloor>\<rfloor> \<in> {X. X = bot \<or> X = null \<or> (\<forall>x\<in>\<lceil>\<lceil>X\<rceil>\<rceil>. x \<noteq> bot)}"
+          apply(frule Set_inv_lemma)
+          apply(simp add: foundation18 invalid_def)
+          done
+
+ have finite_including_rep_set : "\<And>\<tau> X x. \<And>\<tau>. \<tau> \<Turnstile> (\<delta> X and \<upsilon> x) \<Longrightarrow>
+                 finite \<lceil>\<lceil>Rep_Set_0 (X->including(x) \<tau>)\<rceil>\<rceil> = finite \<lceil>\<lceil>Rep_Set_0 (X \<tau>)\<rceil>\<rceil>"
+  apply(rule finite_including_rep_set)
+  apply(metis OclValid_def foundation5)+
+ done
+
+  show "all_defined \<tau> (S->including(x)) \<Longrightarrow> ?thesis"
+   apply(simp add: all_defined_def all_defined_set'_def)
+   apply(erule conjE, frule finite_including_rep_set[of \<tau> S x], simp)
+  by (metis foundation5)
+qed
+
+lemma invert_all_defined' : "(\<forall>\<tau>. all_defined \<tau> (S->including(\<lambda>(_:: '\<AA> st). x))) \<Longrightarrow> is_int (\<lambda> (_:: '\<AA> st). x) \<and> (\<forall>\<tau>. all_defined \<tau> S)"
+   apply(rule conjI)
+   apply(simp only: is_int_def, rule allI)
+   apply(erule_tac x = \<tau> in allE, simp)
+   apply(drule invert_all_defined, simp)
+   apply(rule allI)
+   apply(erule_tac x = \<tau> in allE)
+   apply(drule invert_all_defined, simp)
+done
+
+subsection{* Preservation of cp *}
+
+lemma including_cp_gen : "cp f \<Longrightarrow> cp (\<lambda>r2. ((f r2)->including(x)))"
+ apply(unfold cp_def)
+ apply(subst cp_OclIncluding[of _ x])
+ apply(drule exE) prefer 2 apply assumption
+ apply(rule_tac x = "\<lambda> X_\<tau> \<tau>. ((\<lambda>_. fa X_\<tau> \<tau>)->including(\<lambda>_. x \<tau>)) \<tau>" in exI, simp)
+done
+
+lemma including_cp : "cp (\<lambda>r2. (r2->including(x)))"
+ apply(unfold cp_def)
+ apply(subst cp_OclIncluding[of _ x])
+ apply(rule_tac x = "\<lambda> X_\<tau> \<tau>. ((\<lambda>_. X_\<tau>)->including(\<lambda>_. x \<tau>)) \<tau>" in exI, simp)
+done
+
+lemma including_cp' : "cp (OclIncluding S)"
+ apply(unfold cp_def)
+ apply(subst cp_OclIncluding)
+ apply(rule_tac x = "\<lambda> X_\<tau> \<tau>. ((\<lambda>_. S \<tau>)->including(\<lambda>_. X_\<tau>)) \<tau>" in exI, simp)
+done
+
+lemma including_cp''' : "cp (OclIncluding S->including(i)->including(j))"
+ apply(unfold cp_def)
+ apply(subst cp_OclIncluding)
+ apply(rule_tac x = "\<lambda> X_\<tau> \<tau>. ((\<lambda>_. S->including(i)->including(j) \<tau>)->including(\<lambda>_. X_\<tau>)) \<tau>" in exI, simp)
+done
+
+lemma including_cp2 : "cp (\<lambda>r2. (r2->including(x))->including(y))"
+by(rule including_cp_gen, simp add: including_cp)
+
+lemma including_cp3 : "cp (\<lambda>r2. ((r2->including(x))->including(y))->including(z))"
+by(rule including_cp_gen, simp add: including_cp2)
+
+subsection{* Preservation of global judgment *}
+
+lemma including_cp_all :
+ assumes x_int : "is_int x"
+     and S_def : "\<And>\<tau>. \<tau> \<Turnstile> \<delta> S"
+     and S_incl : "S \<tau>1 = S \<tau>2"
+   shows  "S->including(x) \<tau>1 = S->including(x) \<tau>2"
+proof -
+ have all_defined1 : "\<And>r2 \<tau>. all_defined \<tau> r2 \<Longrightarrow> \<tau> \<Turnstile> \<delta> r2" by(simp add: all_defined_def)
+ show ?thesis
+  apply(unfold OclIncluding_def)
+  apply(simp add:  S_def[simplified OclValid_def] int_is_valid[OF x_int, simplified OclValid_def] S_incl)
+  apply(subgoal_tac "x \<tau>1 = x \<tau>2", simp)
+  apply(insert x_int[simplified is_int_def, THEN spec, of \<tau>1, THEN conjunct2, THEN spec], simp)
+ done
+qed
+
+subsection{* Preservation of non-emptiness *}
+
+lemma including_notempty :
+  assumes S_def : "\<tau> \<Turnstile> \<delta> S"
+      and x_val : "\<tau> \<Turnstile> \<upsilon> x"
+      and S_notempty : "\<lceil>\<lceil>Rep_Set_0 (S \<tau>)\<rceil>\<rceil> \<noteq> {}"
+    shows "\<lceil>\<lceil>Rep_Set_0 (S->including(x) \<tau>)\<rceil>\<rceil> \<noteq> {}"
+proof -
+ have insert_in_Set_0 : "\<And>\<tau>. (\<tau> \<Turnstile>(\<delta> S)) \<Longrightarrow> (\<tau> \<Turnstile>(\<upsilon> x)) \<Longrightarrow> \<lfloor>\<lfloor>insert (x \<tau>) \<lceil>\<lceil>Rep_Set_0 (S \<tau>)\<rceil>\<rceil>\<rfloor>\<rfloor> \<in> {X. X = bot \<or> X = null \<or> (\<forall>x\<in>\<lceil>\<lceil>X\<rceil>\<rceil>. x \<noteq> bot)}"
+          apply(frule Set_inv_lemma)
+          apply(simp add: foundation18 invalid_def)
+          done
+ show ?thesis
+  apply(unfold OclIncluding_def)
+  apply(simp add: S_def[simplified OclValid_def] x_val[simplified OclValid_def] Abs_Set_0_inverse[OF insert_in_Set_0[OF S_def x_val]])
+ done
+qed
+
+lemma including_notempty' :
+  assumes x_val : "\<tau> \<Turnstile> \<upsilon> x"
+    shows "\<lceil>\<lceil>Rep_Set_0 (Set{x} \<tau>)\<rceil>\<rceil> \<noteq> {}"
+proof -
+ have insert_in_Set_0 : "\<And>S \<tau>. (\<tau> \<Turnstile>(\<delta> S)) \<Longrightarrow> (\<tau> \<Turnstile>(\<upsilon> x)) \<Longrightarrow> \<lfloor>\<lfloor>insert (x \<tau>) \<lceil>\<lceil>Rep_Set_0 (S \<tau>)\<rceil>\<rceil>\<rfloor>\<rfloor> \<in> {X. X = bot \<or> X = null \<or> (\<forall>x\<in>\<lceil>\<lceil>X\<rceil>\<rceil>. x \<noteq> bot)}"
+          apply(frule Set_inv_lemma)
+          apply(simp add: foundation18 invalid_def)
+          done
+ show ?thesis
+  apply(unfold OclIncluding_def)
+  apply(simp add: x_val[simplified OclValid_def])
+  apply(subst Abs_Set_0_inverse)
+  apply(rule insert_in_Set_0)
+  apply(simp add: mtSet_all_def)
+  apply(simp_all add: x_val)
+ done
+qed
+
+end
